

1 Universal Constructions

Construction	Definition	Computation	Equality	Commutative Diagram
Initial Object	$\frac{}{0 \xrightarrow{\quad} A}$		$\frac{f:0 \rightarrow A}{f=\quad}$	$0 \xrightarrow{\quad} A$
Terminal Object	$\frac{A}{A \xrightarrow{\quad} 1}$		$\frac{f:A \rightarrow 1}{f=\quad}$	$A \xrightarrow{\quad} 1$
Products	$\frac{A \xrightarrow{f} X \quad A \xrightarrow{g} Y}{A \xrightarrow{\langle f,g \rangle} X \times Y}$	$\pi_1 \circ \langle f, g \rangle = f, \pi_2 \circ \langle f, g \rangle = g$ $\langle \pi_1, \pi_2 \rangle \circ h = h : A \rightarrow X \times Y$	$\frac{\pi_1 \circ h = f : A \rightarrow X \quad \pi_2 \circ h = g : A \rightarrow Y}{h = \langle f, g \rangle : A \rightarrow X \times Y}$	$\begin{array}{ccccc} & & A & & \\ & f \swarrow & \downarrow \langle f,g \rangle & \searrow g & \\ X & \xleftarrow{\pi_1} & X \times Y & \xrightarrow{\pi_2} & Y \end{array}$
Coproducts	$\frac{A \xrightarrow{f} X \quad B \xrightarrow{g} X}{A+B \xrightarrow{[f,g]} X}$	$[f, g] \circ \iota_1 = f, [f, g] \circ \iota_2 = g$ $[h \circ \iota_1, h \circ \iota_2] = h : A + B \rightarrow X$	$\frac{h \circ \iota_1 = f : A \rightarrow X \quad h \circ \iota_2 = g : B \rightarrow X}{h = [f, g] : A + B \rightarrow X}$	$\begin{array}{ccccc} A & \xrightarrow{\iota_1} & A+B & \xleftarrow{\iota_2} & B \\ & f \searrow & \downarrow [f,g] & \swarrow g & \\ & & X & & \end{array}$
Exponentials	$\frac{A \times X \xrightarrow{f} Y}{A \xrightarrow{\text{cur } f} X \Rightarrow Y}$	$\text{app} \circ (\text{cur } f \times \text{id}_X) = f : A \times X \rightarrow Y$ $\text{cur}(\text{app} \circ (h \times \text{id}_X)) = h : A \rightarrow X \Rightarrow Y$	$\frac{\text{app} \circ (h \times \text{id}_X) = f : A \times X \rightarrow Y}{h = \text{cur } f : A \rightarrow X \Rightarrow Y}$	$\begin{array}{ccc} A \times X & \xrightarrow{\text{cur } f \times \text{id}} & (X \Rightarrow Y) \times X \\ & f \searrow & \swarrow \text{app} \\ & & Y \end{array}$
Free monoids	$\frac{X \xrightarrow{f} M \in \text{Set}}{\underline{L}X \xrightarrow{f^\sharp} \underline{M} \in \text{Mon}}$	$f^\sharp \circ s_X = f : X \rightarrow M$ $(g \circ s_X)^\sharp = g : \underline{L}X \rightarrow \underline{M}$	$\frac{h \circ s_X = f : X \rightarrow M}{h = f^\sharp : \underline{L}X \rightarrow \underline{M}}$	$\begin{array}{ccc} X & \xrightarrow{s_X} & \underline{L}X \\ & f \searrow & \downarrow f^\sharp \\ & & \underline{M} \end{array}$

2 Categories

3 Functors

4 Natural Transformations

5 Adjunctions